---
title     : "DataRel: Describing data structures with relations" 
layout    : page
prev      : /Relations/
permalink : /DataRel/
next      : /Equality/
---

```
module plc.vfp.DataRel where
```

In this section we will apply relations to describe properties of the
`List` data type.

## Imports

```
import Relation.Binary.PropositionalEquality as Eq
open Eq using (_≡_; refl; sym; trans; cong)
open Eq.≡-Reasoning
open import Data.Bool using (Bool; true; false; T; _∧_; _∨_; not)
open import Data.Nat using (ℕ; zero; suc; _+_; _*_; _∸_; _≤_; s≤s; z≤n)
open import Data.Nat.Properties using
  (+-assoc; +-identityˡ; +-identityʳ; *-assoc; *-identityˡ; *-identityʳ)
open import Relation.Nullary using (¬_; Dec; yes; no)
open import Data.Product using (_×_; ∃; ∃-syntax) renaming (_,_ to ⟨_,_⟩)
open import Data.List using (List; _∷_; []; _++_; map)
open import Function using (_∘_)
open import plc.vfp.DataProp
open import plc.vfp.Relations using (_⇔_)
```

## Monoids

Typically when we use a fold the operator is associative and the
value is a left and right identity for the operator, meaning that the
operator and the value form a _monoid_.

We can define a monoid as a suitable record type:
```
record IsMonoid {A : Set} (_⊗_ : A → A → A) (e : A) : Set where
  field
    assoc : ∀ (x y z : A) → (x ⊗ y) ⊗ z ≡ x ⊗ (y ⊗ z)
    identityˡ : ∀ (x : A) → e ⊗ x ≡ x
    identityʳ : ∀ (x : A) → x ⊗ e ≡ x

open IsMonoid
```

As examples, sum and zero, multiplication and one, and append and the empty
list, are all examples of monoids:
```
+-monoid : IsMonoid _+_ 0
+-monoid =
  record
    { assoc = +-assoc
    ; identityˡ = +-identityˡ
    ; identityʳ = +-identityʳ
    }

*-monoid : IsMonoid _*_ 1
*-monoid =
  record
    { assoc = *-assoc
    ; identityˡ = *-identityˡ
    ; identityʳ = *-identityʳ
    }

++-monoid : ∀ {A : Set} → IsMonoid {List A} _++_ []
++-monoid =
  record
    { assoc = ++-assoc
    ; identityˡ = ++-identityˡ
    ; identityʳ = ++-identityʳ
    }
```

If `_⊗_` and `e` form a monoid, then we can re-express fold on the
same operator and an arbitrary value:
```
foldr-monoid : ∀ {A : Set} (_⊗_ : A → A → A) (e : A) → IsMonoid _⊗_ e →
  ∀ (xs : List A) (y : A) → foldr _⊗_ y xs ≡ foldr _⊗_ e xs ⊗ y
foldr-monoid _⊗_ e ⊗-monoid [] y =
  begin
    foldr _⊗_ y []
  ≡⟨⟩
    y
  ≡⟨ sym (identityˡ ⊗-monoid y) ⟩
    (e ⊗ y)
  ≡⟨⟩
    foldr _⊗_ e [] ⊗ y
  ∎
foldr-monoid _⊗_ e ⊗-monoid (x ∷ xs) y =
  begin
    foldr _⊗_ y (x ∷ xs)
  ≡⟨⟩
    x ⊗ (foldr _⊗_ y xs)
  ≡⟨ cong (x ⊗_) (foldr-monoid _⊗_ e ⊗-monoid xs y) ⟩
    x ⊗ (foldr _⊗_ e xs ⊗ y)
  ≡⟨ sym (assoc ⊗-monoid x (foldr _⊗_ e xs) y) ⟩
    (x ⊗ foldr _⊗_ e xs) ⊗ y
  ≡⟨⟩
    foldr _⊗_ e (x ∷ xs) ⊗ y
  ∎
```

In a previous exercise we showed the following.
```
postulate
  foldr-++ : ∀ {A : Set} (_⊗_ : A → A → A) (e : A) (xs ys : List A) →
    foldr _⊗_ e (xs ++ ys) ≡ foldr _⊗_ (foldr _⊗_ e ys) xs
```

As a consequence, using a previous exercise, we have the following:
```
foldr-monoid-++ : ∀ {A : Set} (_⊗_ : A → A → A) (e : A) → IsMonoid _⊗_ e →
  ∀ (xs ys : List A) → foldr _⊗_ e (xs ++ ys) ≡ foldr _⊗_ e xs ⊗ foldr _⊗_ e ys
foldr-monoid-++ _⊗_ e monoid-⊗ xs ys =
  begin
    foldr _⊗_ e (xs ++ ys)
  ≡⟨ foldr-++ _⊗_ e xs ys ⟩
    foldr _⊗_ (foldr _⊗_ e ys) xs
  ≡⟨ foldr-monoid _⊗_ e monoid-⊗ xs (foldr _⊗_ e ys) ⟩
    foldr _⊗_ e xs ⊗ foldr _⊗_ e ys
  ∎
```

#### Exercise `foldl` (practice)

Define a function `foldl` which is analogous to `foldr`, but where
operations associate to the left rather than the right.  For example:

    foldr _⊗_ e (x ∷ y ∷ z ∷ [])  =  x ⊗ (y ⊗ (z ⊗ e))
    foldl _⊗_ e (x ∷ y ∷ z ∷ [])  =  ((e ⊗ x) ⊗ y) ⊗ z

```
-- Your code goes here
```


#### Exercise `foldr-monoid-foldl` (practice)

Show that if `_⊗_` and `e` form a monoid, then `foldr _⊗_ e` and
`foldl _⊗_ e` always compute the same result.

```
-- Your code goes here
```


## All {#All}

We can also define predicates over lists. Two of the most important
are `All` and `Any`.

Predicate `All P` holds if predicate `P` is satisfied by every element of a list:
```
data All {A : Set} (P : A → Set) : List A → Set where
  []  : All P []
  _∷_ : ∀ {x : A} {xs : List A} → P x → All P xs → All P (x ∷ xs)
```
The type has two constructors, reusing the names of the same constructors for lists.
The first asserts that `P` holds for every element of the empty list.
The second asserts that if `P` holds of the head of a list and for every
element of the tail of a list, then `P` holds for every element of the list.
Agda uses types to disambiguate whether the constructor is building
a list or evidence that `All P` holds.

For example, `All (_≤ 2)` holds of a list where every element is less
than or equal to two.  Recall that `z≤n` proves `zero ≤ n` for any
`n`, and that if `m≤n` proves `m ≤ n` then `s≤s m≤n` proves `suc m ≤
suc n`, for any `m` and `n`:
```
_ : All (_≤ 2) (0 ∷ 1 ∷ 2 ∷ [])
_ = z≤n ∷ s≤s z≤n ∷ s≤s (s≤s z≤n) ∷ []
```
Here `_∷_` and `[]` are the constructors of `All P` rather than of `List A`.
The three items are proofs of `0 ≤ 2`, `1 ≤ 2`, and `2 ≤ 2`, respectively.

(One might wonder whether a pattern such as `[_,_,_]` can be used to
construct values of type `All` as well as type `List`, since both use
the same constructors. Indeed it can, so long as both types are in
scope when the pattern is declared.  That's not the case here, since
`List` is defined before `[_,_,_]`, but `All` is defined later.)


## Any

Predicate `Any P` holds if predicate `P` is satisfied by some element of a list:
```
data Any {A : Set} (P : A → Set) : List A → Set where
  here  : ∀ {x : A} {xs : List A} → P x → Any P (x ∷ xs)
  there : ∀ {x : A} {xs : List A} → Any P xs → Any P (x ∷ xs)
```
The first constructor provides evidence that the head of the list
satisfies `P`, while the second provides evidence that some element of
the tail of the list satisfies `P`.  For example, we can define list
membership as follows:
```
infix 4 _∈_ _∉_

_∈_ : ∀ {A : Set} (x : A) (xs : List A) → Set
x ∈ xs = Any (x ≡_) xs

_∉_ : ∀ {A : Set} (x : A) (xs : List A) → Set
x ∉ xs = ¬ (x ∈ xs)
```
For example, zero is an element of the list `(0 ∷ 1 ∷ 0 ∷ 2 ∷ [])`.  Indeed, we can demonstrate
this fact in two different ways, corresponding to the two different
occurrences of zero in the list, as the first element and as the third element:
```
_ : 0 ∈ (0 ∷ 1 ∷ 0 ∷ 2 ∷ [])
_ = here refl

_ : 0 ∈ (0 ∷ 1 ∷ 0 ∷ 2 ∷ [])
_ = there (there (here refl))
```
Further, we can demonstrate that three is not in the list, because
any possible proof that it is in the list leads to contradiction:
```
not-in : 3 ∉ (0 ∷ 1 ∷ 0 ∷ 2 ∷ [])
not-in (here ())
not-in (there (here ()))
not-in (there (there (here ())))
not-in (there (there (there (here ()))))
not-in (there (there (there (there ()))))
```
The five occurrences of `()` attest to the fact that there is no
possible evidence for `3 ≡ 0`, `3 ≡ 1`, `3 ≡ 0`, `3 ≡ 2`, and
`3 ∈ []`, respectively.

## All and append

A predicate holds for every element of one list appended to another if and
only if it holds for every element of both lists:
```
All-++-⇔ : ∀ {A : Set} {P : A → Set} (xs ys : List A) →
  All P (xs ++ ys) ⇔ (All P xs × All P ys)
All-++-⇔ xs ys =
  record
    { to       =  to xs ys
    ; from     =  from xs ys
    }
  where

  to : ∀ {A : Set} {P : A → Set} (xs ys : List A) →
    All P (xs ++ ys) → (All P xs × All P ys)
  to [] ys Pys = ⟨ [] , Pys ⟩
  to (x ∷ xs) ys (Px ∷ Pxs++ys) with to xs ys Pxs++ys
  ... | ⟨ Pxs , Pys ⟩ = ⟨ Px ∷ Pxs , Pys ⟩

  from : ∀ { A : Set} {P : A → Set} (xs ys : List A) →
    All P xs × All P ys → All P (xs ++ ys)
  from [] ys ⟨ [] , Pys ⟩ = Pys
  from (x ∷ xs) ys ⟨ Px ∷ Pxs , Pys ⟩ =  Px ∷ from xs ys ⟨ Pxs , Pys ⟩
```

#### Exercise `Any-++-⇔` (recommended)

Prove a result similar to `All-++-⇔`, but with `Any` in place of `All`, and a suitable
replacement for `_×_`.  As a consequence, demonstrate an equivalence relating
`_∈_` and `_++_`.

```
-- Your code goes here
```

#### Exercise `All-++-≃` (stretch)

Show that the equivalence `All-++-⇔` can be extended to an isomorphism.

```
-- Your code goes here
```

#### Exercise `¬Any⇔All¬` (recommended)

Show that `Any` and `All` satisfy a version of De Morgan's Law:

    (¬_ ∘ Any P) xs ⇔ All (¬_ ∘ P) xs

(Can you see why it is important that here `_∘_` is generalised
to arbitrary levels, as described in the section on
[universe polymorphism]({{ site.baseurl }}/Equality/#unipoly)?)

Do we also have the following?

    (¬_ ∘ All P) xs ⇔ Any (¬_ ∘ P) xs

If so, prove; if not, explain why.


```
-- Your code goes here
```

#### Exercise `¬Any≃All¬` (stretch)

Show that the equivalence `¬Any⇔All¬` can be extended to an isomorphism.
You will need to use extensionality.

```
-- Your code goes here
```

#### Exercise `All-∀` (practice)

Show that `All P xs` is isomorphic to `∀ {x} → x ∈ xs → P x`.

```
-- You code goes here
```


#### Exercise `Any-∃` (practice)

Show that `Any P xs` is isomorphic to `∃[ x ] (x ∈ xs × P x)`.

```
-- You code goes here
```


## Decidability of All

If we consider a predicate as a function that yields a boolean,
it is easy to define an analogue of `All`, which returns true if
a given predicate returns true for every element of a list:
```
all : ∀ {A : Set} → (A → Bool) → List A → Bool
all p  =  foldr _∧_ true ∘ map p
```
The function can be written in a particularly compact style by
using the higher-order functions `map` and `foldr`.

As one would hope, if we replace booleans by decidables there is again
an analogue of `All`.  First, return to the notion of a predicate `P` as
a function of type `A → Set`, taking a value `x` of type `A` into evidence
`P x` that a property holds for `x`.  Say that a predicate `P` is _decidable_
if we have a function that for a given `x` can decide `P x`:
```
Decidable : ∀ {A : Set} → (A → Set) → Set
Decidable {A} P  =  ∀ (x : A) → Dec (P x)
```
Then if predicate `P` is decidable, it is also decidable whether every
element of a list satisfies the predicate:
```
All? : ∀ {A : Set} {P : A → Set} → Decidable P → Decidable (All P)
All? P? []                                 =  yes []
All? P? (x ∷ xs) with P? x   | All? P? xs
...                 | yes Px | yes Pxs     =  yes (Px ∷ Pxs)
...                 | no ¬Px | _           =  no λ{ (Px ∷ Pxs) → ¬Px Px   }
...                 | _      | no ¬Pxs     =  no λ{ (Px ∷ Pxs) → ¬Pxs Pxs }
```
If the list is empty, then trivially `P` holds for every element of
the list.  Otherwise, the structure of the proof is similar to that
showing that the conjunction of two decidable propositions is itself
decidable, using `_∷_` rather than `⟨_,_⟩` to combine the evidence for
the head and tail of the list.


#### Exercise `Any?` (stretch)

Just as `All` has analogues `all` and `All?` which determine whether a
predicate holds for every element of a list, so does `Any` have
analogues `any` and `Any?` which determine whether a predicate holds
for some element of a list.  Give their definitions.

```
-- Your code goes here
```


#### Exercise `split` (stretch)

The relation `merge` holds when two lists merge to give a third list.
```
data merge {A : Set} : (xs ys zs : List A) → Set where

  [] :
      --------------
      merge [] [] []

  left-∷ : ∀ {x xs ys zs}
    → merge xs ys zs
      --------------------------
    → merge (x ∷ xs) ys (x ∷ zs)

  right-∷ : ∀ {y xs ys zs}
    → merge xs ys zs
      --------------------------
    → merge xs (y ∷ ys) (y ∷ zs)
```

For example,
```
_ : merge (1 ∷ 4 ∷ []) (2 ∷ 3 ∷ []) (1 ∷ 2 ∷ 3 ∷ 4 ∷ [])
_ = left-∷ (right-∷ (right-∷ (left-∷ [])))

```

Given a decidable predicate and a list, we can split the list
into two lists that merge to give the original list, where all
elements of one list satisfy the predicate, and all elements of
the other do not satisfy the predicate.

Define the following variant of the traditional `filter` function on
lists, which given a decidable predicate and a list returns a list of
elements that satisfy the predicate and a list of elements that don't,
with their corresponding proofs.

    split : ∀ {A : Set} {P : A → Set} (P? : Decidable P) (zs : List A)
      → ∃[ xs ] ∃[ ys ] ( merge xs ys zs × All P xs × All (¬_ ∘ P) ys )

```
-- Your code goes here
```

## Standard Library

Definitions similar to those in this section can be found in the standard library:
```
import Data.List using (List; _++_; length; reverse; map; foldr; downFrom)
import Data.List.All using (All; []; _∷_)
import Data.List.Any using (Any; here; there)
import Data.List.Membership.Propositional using (_∈_)
import Data.List.Properties
  using (reverse-++-commute; map-compose; map-++-commute; foldr-++)
  renaming (mapIsFold to map-is-foldr)
import Algebra.Structures using (IsMonoid)
import Relation.Unary using (Decidable)
import Relation.Binary using (Decidable)
```
The standard library version of `IsMonoid` differs from the
one given here, in that it is also parameterised on an equivalence relation.

Both `Relation.Unary` and `Relation.Binary` define a version of `Decidable`,
one for unary relations (as used in this section where `P` ranges over
unary predicates) and one for binary relations (as used earlier, where `_≤_`
ranges over a binary relation).

## Unicode

This section uses the following Unicode symbols:

    ∷  U+2237  PROPORTION  (\::)
    ⊗  U+2297  CIRCLED TIMES  (\otimes, \ox)
    ∈  U+2208  ELEMENT OF  (\in)
    ∉  U+2209  NOT AN ELEMENT OF  (\inn, \notin)

---

*This page is derived from Wadler et al.; for more information see the [sources and authorship]({{ site.baseurl }}/Sources/) page.*
